FIX support for value categories.

auto-theories/auto/Lemmas/Wp.v
@@ -19,169 +19,302 @@ Section with_resolve.
   Context {resolve : genv}.
   Context (ti : thread_info) (ρ : region).
 
-  Notation wp_rhs := (@wp_rhs resolve ti ρ).
-  Notation wp_lhs := (@wp_lhs resolve ti ρ).
+  Notation wp_prval := (@wp_prval resolve ti ρ).
+  Notation wp_rval := (@wp_rval resolve ti ρ).
+  Notation wp_lval := (@wp_lval resolve ti ρ).
+  Notation wp_xval := (@wp_xval resolve ti ρ).
+  Notation wp_args := (@wp_args resolve ti ρ).
+  Notation wp_init := (@wp_init resolve ti ρ).
   Notation wp := (@wp resolve ti ρ).
   Notation wp_decl := (@wp_decl resolve ti ρ).
   Notation wp_eval_binop := (@wp_eval_binop resolve).
   Notation wp_eval_unop := (@wp_eval_unop resolve).
 
-Lemma wp_rhs_local (ty : type) : forall x Q,
-    Exists v, (tlocal ρ x (tprim (drop_qualifiers ty) v) ** ltrue) //\\ Q v empSP
-    |-- wp_rhs (Ecast Cl2r (Lvalue, Evar (Lname x) ty) ty) Q.
-Proof.
-  unfold tlocal. intros.
-  work.
-  rewrite bilexistsscL2.
-  rewrite landexistsD1.
-  work.
-  rewrite <- wp_rhs_cast_l2r.
-  rewrite <- wp_lhs_lvar.
-  work.
-  { eapply landL1.
-    unfold tlocal_at.
-    rewrite sepSPA.
-    eapply scME. reflexivity. eapply ltrueR. }
-  { unfold tlocal_at; simpl.
-    eapply landL1.
-    instantiate (1:=v).
-    work. }
-  { eapply landL2. reflexivity. }
-Qed.
+  Definition find_constant (nm : globname) (m : compilation_unit) : option Expr :=
+    match CompilationUnit.lookup_global m nm with
+    | Some (Gconstant _ e) => Some e
+    | _ => None
+    end.
 
-(* this is the common case for member access
- *)
-Lemma wp_rhs_dot : forall obj f fty z Q,
-    wp_lhs obj (fun base free =>
+  Definition find_struct (nm : globname) (m : compilation_unit) : option Struct :=
+    match CompilationUnit.lookup_global m nm with
+    | Some (Gstruct s) => Some s
+    | _ => None
+    end.
 
-       Exists val,
-         (_at (_offsetL (_field f) (_eq base)) (tprim (drop_qualifiers fty) val) ** ltrue) //\\
-       Q val free)
-    |-- wp_rhs (Ecast Cl2r (Lvalue, Emember obj f fty) z) Q.
-Proof. Admitted.
+  Theorem find_struct_ok : forall nm m s,
+      find_struct nm m = Some s ->
+      denoteModule m |-- denoteModule m ** denoteGlobal nm (Gstruct s).
+  Proof.
+    destruct m; simpl.
+    unfold find_struct. unfold lookup_global.
+    intros.
+    simpl in *.
+    unfold denoteModule. simpl.
+    work.
+  Qed.
 
-Lemma wp_lhs_assign_member_ignore : forall f t obj e t' Q,
-    wp_lhs obj (fun base free =>
-    wp_rhs e (fun v' free' =>
-        _at (_offsetL (_field f) (_eq base)) (uninit (drop_qualifiers t)) **
-        (_at (_offsetL (_field f) (_eq base)) (tprim (drop_qualifiers t) v') -*
-        Q (free ** free'))))
-    |-- wp_lhs (Eassign (Emember obj f t) e t') (fun _ free => Q free).
-Proof. Admitted.
+  (* accessing constants *)
+  Theorem wp_prval_const : forall m ty cnst e Q R P,
+    P |-- denoteModule m ** ltrue ->
+    find_constant cnst m = Some e ->
+    P |-- wp_prval e Q ** R ->
+    P |-- wp_prval (Econst_ref (Gname cnst) ty) Q ** R.
+  Proof.
+    intros.
+  Admitted.
+
+  (* Variable access *)
+  Theorem wp_prval_cast_l2r_l : forall ty e Q,
+      wp_lval e (fun a free =>
+           Exists v, (_at (_eq a) (tprim (erase_qualifiers ty) v) **
+                     (_at (_eq a) (tprim (erase_qualifiers ty) v) -* Q v free)))
+      |-- wp_prval (Ecast Cl2r (Lvalue, e) ty) Q.
+  Proof.
+    intros. rewrite <- wp_prval_cast_l2r_l.
+    eapply Proper_wp_lval. red. red. intros.
+    eapply lexists_lentails_m. intro.
+    work.
+    admit. (* perm_left ltac:(idtac; perm_right ltac:(idtac; eapply wand_apply)).
+    work. *)
+  Admitted.
+
+  Theorem wp_prval_cast_l2r_x : forall ty e Q,
+      wp_xval e (fun a free =>
+                   Exists v, (_at (_eq a) (tprim (erase_qualifiers ty) v) **
+                             (_at (_eq a) (tprim (erase_qualifiers ty) v) -* Q v free)))
+      |-- wp_prval (Ecast Cl2r (Xvalue, e) ty) Q.
+  Proof.
+    intros. rewrite <- wp_prval_cast_l2r_x.
+    eapply Proper_wp_xval. red. red. intros.
+    eapply lexists_lentails_m. intro.
+    work.
+    admit. (* perm_left ltac:(idtac; perm_right ltac:(idtac; eapply wand_apply)).
+    work. *)
+  Admitted.
+
+  Lemma wp_prval_local (ty : type) : forall x Q,
+    Exists p, Exists v,
+      tlocal_at ρ x p (tprim (erase_qualifiers ty) v) **
+      (tlocal_at ρ x p (tprim (erase_qualifiers ty) v) -* Q v empSP)
+    |-- wp_prval (Ecast Cl2r (Lvalue, Evar (Lname x) ty) ty) Q.
+  Proof.
+    intros. unfold tlocal_at.
+    work.
+    rewrite <- wp_prval_cast_l2r_l.
+    rewrite <- wp_lval_lvar.
+    work.
+    rewrite (sepSPC (addr_of _ _)), sepSPA.
+    apply wandSPL; work.
+  Qed.
+
+  (* this is the common case for member access
+   *)
+  Lemma wp_prval_dot : forall obj f fty z Q,
+      wp_lval obj (fun base free => Exists val,
+         (_at (_offsetL (_field f) (_eq base)) (tprim (erase_qualifiers fty) val) **
+         (_at (_offsetL (_field f) (_eq base)) (tprim (erase_qualifiers fty) val) -*
+          Q val free)))
+      |-- wp_prval (Ecast Cl2r (Lvalue, Emember obj f fty) z) Q.
+  Proof.
+    intros. rewrite <- wp_prval_cast_l2r_l. rewrite <- wp_lval_member.
+    apply Proper_wp_lval. intro. intro. work.
+    - admit.
+    - admit.
+  Admitted.
 
 
-Lemma wp_lhs_assign_member : forall f t obj e t' Q,
-    wp_lhs obj (fun base free =>
-    wp_rhs e (fun v' free' =>
-        Exists addr, (_offsetL (_field f) (_eq base) &~ addr ** ltrue) //\\
-        _at (_eq addr) (tany (drop_qualifiers t)) **
-        (_at (_eq addr) (tprim (drop_qualifiers t) v') -* Q addr (free ** free'))))
-    |-- wp_lhs (Eassign (Emember obj f t) e t') Q.
-Proof. Admitted.
+  (* member assignment *)
+  Lemma wp_lval_assign_member_ignore : forall f t obj e t' Q,
+      wp_lval obj (fun base free => wp_prval e (fun v' free' =>
+         _at (_offsetL (_field f) (_eq base)) (uninit (erase_qualifiers t)) **
+        (_at (_offsetL (_field f) (_eq base)) (tprim (erase_qualifiers t) v') -*
+         Q (free ** free'))))
+      |-- wp_lval (Eassign (Emember obj f t) e t') (fun _ free => Q free).
+  Proof. Admitted.
+
+  Lemma wp_lval_assign_member : forall f t obj e t' Q,
+      wp_lval obj (fun base free => wp_prval e (fun v' free' =>
+         Exists addr, (_offsetL (_field f) (_eq base) &~ addr ** ltrue) //\\
+           _at (_eq addr) (tany (erase_qualifiers t)) **
+           (_at (_eq addr) (tprim (erase_qualifiers t) v') -* Q addr (free ** free'))))
+      |-- wp_lval (Eassign (Emember obj f t) e t') Q.
+  Proof. Admitted.
+
+  (* casting *)
+  Theorem wp_prval_cast_tovoid : forall vc e ty Q,
+      wpe (resolve:=resolve) ti ρ vc e (fun _ => Q (Vint 0))
+      |-- wp_prval (Ecast C2void (vc,e) ty) Q.
+  Proof.
+    intros. etransitivity; [ | eapply  wpe_cast_tovoid with (vc':=Rvalue) ].
+    reflexivity.
+  Qed.
+
+  Theorem wp_rval_xval_materialize : forall ty e Q,
+    wp_xval (Ematerialize_temp e ty) Q
+    |-- wp_rval (Ematerialize_temp e ty) Q.
+  Proof. intros. eapply lorR2. reflexivity. Qed.
 
 
-Theorem wp_call_glob : forall vc f ret ts es K PQ F F' ty ty' ty'',
-   (vc = Lvalue \/ vc = Rvalue) ->
-   F |-- (|> cglob (resolve:=resolve) f ti (SFunction ret ts PQ)) ** ltrue ->
-   F
-   |-- wps (wpAnys (resolve:=resolve) ti ρ) es (fun vs free => applyEach ts vs PQ (fun wpp _ =>
-            WppD wpp (fun r => K r free))) empSP ** F' ->
-   F
-   |-- wp_rhs
-         (Ecall (Ecast Cfunction2pointer (vc, Evar (Gname f) ty) ty') es ty'')
-         K ** F'.
-Proof. Admitted.
+  (* function calls *)
+  Theorem wp_prval_call_glob : forall vc f ret ts es K PQ F F' ty ty' ty'',
+      match vc with
+      | Lvalue | Rvalue => True
+      | _ => False
+      end ->
+      F |-- (|> cglob (resolve:=resolve) f ti (SFunction ret ts PQ)) ** ltrue ->
+      F |-- wp_args es (fun vs free => applyEach ts vs PQ (fun wpp _ =>
+               WppD wpp (fun r => K r free))) ** F' ->
+      F |-- wp_prval (Ecall (Ecast Cfunction2pointer (vc, Evar (Gname f) ty) ty') es ty'')
+                     K ** F'.
+  (* note(gmm): this incorporates both the C and the C++ calling rules *)
+  Proof. Admitted.
 
-Lemma wp_member_call_glob:
-  forall (gn : globname) this (ret : type)
-    ty
-    (ts : list type) es (K : val -> FreeTemps -> mpred)
-    (PQ : val -> arrowFrom val ts WithPrePost) (F F' : mpred)
-    cls q,
-    F |-- (|> cglob (resolve:=resolve) gn ti (SMethod cls q ret ts PQ)) ** ltrue ->
-    F
-    |-- wp_lhs this (fun this =>
-          wps (wpAnys (resolve:=resolve) ti ρ) es (fun (vs : list val) free =>
-            applyEach ts vs (PQ this) (fun wpp _ =>
-              WppD wpp (fun r => K r free)))) ** F' ->
-    F
-    |-- wp_rhs (Emember_call false gn this es ty) K ** F'.
-Proof. Admitted.
+  Theorem wp_xval_call_glob : forall vc f ret ts es K PQ F F' ty ty' ty'',
+      match vc with
+      | Lvalue | Rvalue => True
+      | _ => False
+      end ->
+      F |-- (|> cglob (resolve:=resolve) f ti (SFunction ret ts PQ)) ** ltrue ->
+      F |-- wp_args es (fun vs free => applyEach ts vs PQ (fun wpp _ =>
+               WppD wpp (fun r => K r free))) ** F' ->
+      F |-- wp_xval (Ecall (Ecast Cfunction2pointer (vc, Evar (Gname f) ty) ty') es ty'')
+                    K ** F'.
+  (* note(gmm): this incorporate both the C and the C++ calling rules *)
+  Proof. Admitted.
 
-Theorem wp_constructor_glob : forall cname cls ts es K PQ F F' ty,
-   F |-- (|> cglob (resolve:=resolve) cname ti (SConstructor cls ts PQ)) ** ltrue ->
-   F
-   |-- wps (wpAnys (resolve:=resolve) ti ρ) es (fun vs free =>
-             (* note(gmm): this is cancelling the `uninitialized_ty`
-              * which is inserted into the pre-condition by `SConstructor` *)
-             Forall a, applyEach ts vs (PQ a) (fun wpp _ =>
-               WppD wpp (fun _ => K a free))) empSP ** F' ->
-   F
-   |-- wp_rhs (Econstructor cname es ty) K ** F'.
-Proof.
+  Theorem wp_init_call_glob:
+    forall (vc : ValCat)
+      (f : globname) (ret : type) (ts : list type) (es : list (ValCat * Expr))
+      (K : FreeTemps -> mpred) (PQ : arrowFrom val ts WithPrePost) addr
+      (F F' : mpred) (ty ty' ty'' ty''' : type),
+      match vc with
+      | Xvalue => False
+      | _ => True
+      end ->
+      F |-- (|> cglob (resolve:=resolve) f ti (SFunction ret ts PQ)) ** ltrue ->
+      F |-- wp_args es (fun (vs : list val) (free : FreeTemps) =>
+           applyEach ts vs PQ
+                     (fun (wpp : WithPrePost) (_ : list (type * val)) =>
+                        _at (_eq addr) (uninit (erase_qualifiers ty''')) **
+                            WppD wpp (fun r : val => [| r = addr |] -* K free))) ** F' ->
+      F |-- wp_init ty''' addr
+        (Ecall (Ecast Cfunction2pointer (vc, Evar (Gname f) ty) ty') es ty'') K ** F'.
+  Proof. Admitted.
+
+  (* member calls (non-virtual) *)
+  Lemma wp_prval_member_call_glob:
+    forall (gn : globname) this (ret : type)
+      ty
+      (ts : list type) es (K : val -> FreeTemps -> mpred)
+      (PQ : val -> arrowFrom val ts WithPrePost) (F F' : mpred)
+      cls q,
+      F |-- (|> cglob (resolve:=resolve) gn ti (SMethod cls q ret ts PQ)) ** ltrue ->
+      F |-- wp_lval this (fun this free' => wp_args es (fun (vs : list val) free =>
+               applyEach ts vs (PQ this) (fun wpp _ =>
+                    WppD wpp (fun r => free' ** K r free)))) ** F' ->
+      F |-- wp_prval (Emember_call false gn this es ty) K ** F'.
+  Proof. Admitted.
+
+  Lemma wp_xval_member_call_glob:
+    forall (gn : globname) this (ret : type)
+      ty
+      (ts : list type) es (K : val -> FreeTemps -> mpred)
+      (PQ : val -> arrowFrom val ts WithPrePost) (F F' : mpred)
+      cls q,
+      F |-- (|> cglob (resolve:=resolve) gn ti (SMethod cls q ret ts PQ)) ** ltrue ->
+      F |-- wp_lval this (fun this free' => wp_args es (fun (vs : list val) free =>
+               applyEach ts vs (PQ this) (fun wpp _ =>
+                    WppD wpp (fun r => free' ** K r free)))) ** F' ->
+      F |-- wp_xval (Emember_call false gn this es ty) K ** F'.
+  Proof. Admitted.
+
+  Theorem wp_init_member_call_glob:
+    forall (vc : ValCat)
+      (f : obj_name) this (ret : type) (ts : list type) (es : list (ValCat * Expr))
+      (K : FreeTemps -> mpred) (PQ : arrowFrom val ts WithPrePost) addr
+      (F F' : mpred) (ty ty' : type),
+      match vc with
+      | Xvalue => False
+      | _ => True
+      end ->
+      F |-- (|> cglob (resolve:=resolve) f ti (SFunction ret ts PQ)) ** ltrue ->
+      F |-- wp_args es (fun (vs : list val) (free : FreeTemps) =>
+           applyEach ts vs PQ
+                     (fun (wpp : WithPrePost) (_ : list (type * val)) =>
+                        _at (_eq addr) (uninit (erase_qualifiers ty')) **
+                            WppD wpp (fun r : val => [| r = addr |] -* K free))) ** F' ->
+      F |-- wp_init ty' addr (Emember_call false f this es ty) K ** F'.
+  Proof. Admitted.
+
+  (* constructors *)
+  Theorem wp_init_ctor_glob : forall loc cname cls ts es K PQ F F' ty,
+      F |-- (|> cglob (resolve:=resolve) cname ti (SConstructor cls ts PQ)) ** ltrue ->
+      F |-- wp_args es (fun vs free => applyEach ts vs (PQ loc) (fun wpp _ =>
+               _at (_eq loc) (uninit (Tref cls)) **
+               (* ^ note: this is because SConstructor inserts the
+                * [uninit] fact, so we have to add it here *)
+               WppD wpp (fun _ => K free))) ** F' ->
+      F |-- wp_init (Tref cls) loc (Econstructor cname es ty) K ** F'.
+  Proof. Admitted.
+
+  (* destructors *)
+  Theorem wp_destroy
+    : forall this cls F F' Q PQ' dt,
+      F |-- (|> cglob (resolve:=resolve) dt ti (SDestructor cls PQ')) ** ltrue ->
+      F |-- (WppD (PQ' this) (fun _ => Q) ** F') ->
+      F |-- destruct_obj (resolve:=resolve) ti dt cls this Q ** F'.
+  Proof. Admitted.
+
+  (* todo(gmm): destroy an array? *)
+
+  (* declarations *)
+  Theorem wp_decl_class_dtor
+    : forall x ty es cls cname (k : Kpreds -> mpred) ts PQ F F' Q PQ' dtor,
+      F |-- (|> cglob (resolve:=resolve) cname ti (SConstructor cls ts PQ)) ** ltrue ->
+      F |-- (|> cglob (resolve:=resolve) dtor ti (SDestructor cls PQ')) ** ltrue ->
+      F |-- wp_args es (fun vs free =>
+               (* note(gmm): this is cancelling the `uninitialized_ty`
+                * which is inserted into the pre-condition by `SConstructor` *)
+               Forall a, applyEach ts vs (PQ a) (fun wpp _ =>
+                 WppD wpp (fun _ => free ** (_local ρ x &~ a -* k (Kat_exit (fun Q' =>
+                     let wpp := PQ' a in
+                     WppD wpp (fun _ =>
+                             (* note(gmm): this is canceling the dead memory
+                              * that is inserted by `SDestructor` *)
+                             _local ρ x &~ a ** Q')) Q))))) ** F' ->
+      F |-- wp_decl x (Tref cls) (Some (Econstructor cname es ty)) (Some dtor) k Q ** F'.
+  Proof. Admitted.
+
+  Theorem wp_decl_class_no_dtor
+    : forall x ty es cls cname (k : Kpreds -> mpred) ts PQ F F' Q,
+      F |-- (|> cglob (resolve:=resolve) cname ti (SConstructor cls ts PQ)) ** ltrue ->
+      F |-- wp_args es (fun vs free =>
+               (* note(gmm): this is cancelling the `uninitialized_ty`
+                * which is inserted into the pre-condition by `SConstructor` *)
+               Forall a, applyEach ts vs (PQ a) (fun wpp _ =>
+                 WppD wpp
+                      (fun _ => free ** (_local ρ x &~ a -* k (Kat_exit (fun Q' =>
+                                                                        _local ρ x &~ a ** _at (_eq a) (tany (Tref cls)) ** Q') Q))))) ** F' ->
+      F |-- wp_decl x (Tref cls) (Some (Econstructor cname es ty)) None k Q ** F'.
+  Proof. Admitted.
+
 (*
-      intros.
-      rewrite H; clear H.
-      rewrite <- wp_call.
-      rewrite <- wp_rhs_cast_function2pointer.
-      simplify_wp.
-      unfold cglob.
-      discharge ltac:(canceler fail eauto) eauto.
-      rewrite wps_frame.
-      rewrite sepSPC.
-      rewrite wps_frame.
-      eapply Proper_wps_entails; eauto.
-      red. intros.
-      rewrite sepSPC.
-      etransitivity.
-      eapply triple'_apply with (vs:=a).
-      reflexivity.
-      discharge auto.
-      eapply spec_later_weaken.
-*)
-Admitted.
 
-Theorem wp_decl_class
-: forall x ty es cls cname (k : Kpreds -> mpred) ts PQ F F' Q dname PQ',
-    F |-- (|> cglob (resolve:=resolve) cname ti (SConstructor cls ts PQ)) ** ltrue ->
-    F |-- (|> cglob (resolve:=resolve) dname ti (SDestructor cls PQ')) ** ltrue ->
-    F
-    |-- wps (wpAnys (resolve:=resolve) ti ρ) es (fun vs free =>
-             (* note(gmm): this is cancelling the `uninitialized_ty`
-              * which is inserted into the pre-condition by `SConstructor` *)
-             Forall a, applyEach ts vs (PQ a) (fun wpp _ =>
-               WppD wpp
-                    (fun _ => free ** (_local ρ x &~ a -* k (Kat_exit (fun Q' =>
-                       WppD (PQ' a)
-                            (fun _ =>
-                               (* note(gmm): this is canceling the dead memory
-                                * that is inserted by `SDestructor` *)
-                               _local ρ x &~ a ** Q')) Q))))) empSP ** F' ->
-    F
-    |-- wp_decl x (Tref cls) (Some (Econstructor cname es ty)) k Q ** F'.
-Proof. Admitted.
+(** STOPPED *)
 
-Theorem wp_destroy
-: forall this cls F F' Q PQ' dt,
-    F |-- (|> cglob (resolve:=resolve) (dtor_name dt cls) ti (SDestructor cls PQ')) ** ltrue ->
-    F
-    |-- (WppD (PQ' this) (fun _ => Q) ** F') ->
-    F
-    |-- destroy (resolve:=resolve) ti dt cls this Q ** F'.
-Proof. Admitted.
-
-Lemma wp_rhs_cast_noop:
+Lemma wp_prval_cast_noop:
   forall (ty : type) (e : Expr) (Q : val -> FreeTemps -> mpred),
-  wp_rhs e Q |-- wp_rhs (Ecast Cnoop (Rvalue, e) ty) Q.
+  wp_prval e Q |-- wp_prval (Ecast Cnoop (Rvalue, e) ty) Q.
 Proof. intros. eapply wpe_cast_noop with (m:=Rvalue). Qed.
 
-Lemma wp_lhs_cast_noop:
+Lemma wp_lval_cast_noop:
   forall (ty : type) (e : Expr) (Q : val -> FreeTemps -> mpred),
-  wp_lhs e Q |-- wp_lhs (Ecast Cnoop (Lvalue, e) ty) Q.
+  wp_lval e Q |-- wp_lval (Ecast Cnoop (Lvalue, e) ty) Q.
 Proof. intros; eapply wpe_cast_noop with (m:=Lvalue). Qed.
 
 Theorem wp_decl_reference : forall x ty init k Q,
-    wp_lhs init (fun a free => _local ρ x &~ a -* (free ** k (Kfree (_local ρ x &~ a) Q)))
+    wp_lval init (fun a free => _local ρ x &~ a -* (free ** k (Kfree (_local ρ x &~ a) Q)))
     |-- wp_decl x (Treference ty) (Some init) k Q.
 Proof. reflexivity. Qed.
 
@@ -192,7 +325,7 @@ Theorem wp_decl_pointer : forall x ty init k Q,
       Forall a, tlocal_at ρ x a (uninit (Tpointer ty))
               -* k (Kfree (tlocal ρ x (tany (Tpointer ty))) Q)
     | Some init =>
-      wp_rhs init (fun v free =>
+      wp_prval init (fun v free =>
                  Forall a, tlocal_at ρ x a (tprim (Tpointer ty) v)
               -* (free ** k (Kfree (tlocal ρ x (tany (Tpointer ty))) Q)))
     end
@@ -200,7 +333,7 @@ Theorem wp_decl_pointer : forall x ty init k Q,
 Proof.
   simpl; intros. unfold tlocal.
   destruct init.
-  { eapply Proper_wp_rhs. red. red. intros.
+  { eapply Proper_wp_prval. red. red. intros.
     work.
     eapply wandSPE.
     2:{ eapply sepSPC. }
@@ -220,7 +353,7 @@ Theorem wp_decl_int : forall x a b init k Q,
     | None =>
       tlocal ρ x (uninit (Tint a b)) -* k (Kfree (tlocal ρ x (tany (Tint a b))) Q)
     | Some init =>
-      wp_rhs init (fun v free =>
+      wp_prval init (fun v free =>
                  tlocal ρ x (tprim (Tint a b) v)
               -* (free ** k (Kfree (tlocal ρ x (tany (Tint a b))) Q)))
     end
@@ -232,7 +365,7 @@ Theorem wp_decl__int : forall x init k Q,
     | None =>
       tlocal ρ x (uninit T_int) -* k (Kfree (tlocal ρ x (tany T_int)) Q)
     | Some init =>
-      wp_rhs init (fun v free =>
+      wp_prval init (fun v free =>
                  tlocal ρ x (tprim T_int v)
               -* (free ** k (Kfree (tlocal ρ x (tany T_int)) Q)))
     end
@@ -244,7 +377,7 @@ Theorem wp_decl__ulong : forall x init k Q,
     | None =>
       tlocal ρ x (uninit T_ulong) -* k (Kfree (tlocal ρ x (tany T_ulong)) Q)
     | Some init =>
-      wp_rhs init (fun v free =>
+      wp_prval init (fun v free =>
                  tlocal ρ x (tprim T_ulong v)
               -* (free ** k (Kfree (tlocal ρ x (tany T_ulong)) Q)))
     end
@@ -256,7 +389,7 @@ Theorem wp_decl__int32 : forall x init k Q,
     | None =>
       tlocal ρ x (uninit T_int32) -* k (Kfree (tlocal ρ x (tany T_int32)) Q)
     | Some init =>
-      wp_rhs init (fun v free =>
+      wp_prval init (fun v free =>
                  tlocal ρ x (tprim T_int32 v)
               -* (free ** k (Kfree (tlocal ρ x (tany T_int32)) Q)))
     end
@@ -269,7 +402,7 @@ Theorem wp_decl_char : forall x a b init k Q,
     | None =>
       tlocal ρ x (uninit (Tchar a b)) -* k (Kfree clean Q)
     | Some init =>
-      wp_rhs init (fun v free =>
+      wp_prval init (fun v free =>
                  tlocal ρ x (tprim (Tchar a b) v)
               -* (free ** k (Kfree clean Q)))
     end)
@@ -282,7 +415,7 @@ Theorem wp_decl_bool : forall x init k Q,
     | None =>
       tlocal ρ x (uninit Tbool) -* clean
     | Some init =>
-      wp_rhs init (fun v free =>
+      wp_prval init (fun v free =>
                  tlocal ρ x (tprim Tbool v)
               -* (free ** clean))
     end)
@@ -305,20 +438,20 @@ Theorem wp_decl_mut : forall x ty init k Q,
 Proof. reflexivity. Qed.
 
 (* conditions *)
-Lemma wp_lhs_condition : forall ty tst th el Q,
-    wp_rhs tst (fun v1 free =>
+Lemma wp_lval_condition : forall ty tst th el Q,
+    wp_prval tst (fun v1 free =>
        if is_true v1
-       then wp_lhs th (fun v free' => Q v (free ** free'))
-       else wp_lhs el (fun v free' => Q v (free ** free')))
-    |-- wp_lhs (Eif tst th el ty) Q.
+       then wp_lval th (fun v free' => Q v (free ** free'))
+       else wp_lval el (fun v free' => Q v (free ** free')))
+    |-- wp_lval (Eif tst th el ty) Q.
 Proof. intros; eapply wp_condition with (m:=Lvalue). Qed.
 
-Lemma wp_rhs_condition : forall ty tst th el Q,
-    wp_rhs tst (fun v1 free =>
+Lemma wp_prval_condition : forall ty tst th el Q,
+    wp_prval tst (fun v1 free =>
       if is_true v1
-      then wp_rhs th (fun v free' => Q v (free ** free'))
-      else wp_rhs el (fun v free' => Q v (free ** free')))
-    |-- wp_rhs (Eif tst th el ty) Q.
+      then wp_prval th (fun v free' => Q v (free ** free'))
+      else wp_prval el (fun v free' => Q v (free ** free')))
+    |-- wp_prval (Eif tst th el ty) Q.
 Proof. intros; eapply wp_condition with (m:=Rvalue). Qed.
 
 Lemma wp_skip : forall (Q : Kpreds),
@@ -326,140 +459,144 @@ Lemma wp_skip : forall (Q : Kpreds),
 Proof. unfold Sskip. intros. rewrite <- wp_seq. reflexivity. Qed.
 
 Lemma wp_return_lhs : forall Q e,
-    wp_lhs e (finish (fun res : val => k_return Q (Some res)))
+    wp_lval e (finish (fun res : val => k_return Q (Some res)))
     |-- wp (Sreturn (Some (Lvalue, e))) Q.
 Proof. intros. eapply wp_return_val with (c:=Lvalue). Qed.
 
 Lemma wp_return_rhs : forall Q e,
-    wp_rhs e (finish (fun res : val => k_return Q (Some res)))
+    wp_prval e (finish (fun res : val => k_return Q (Some res)))
     |-- wp (Sreturn (Some (Rvalue, e))) Q.
 Proof. intros. eapply wp_return_val with (c:=Rvalue). Qed.
 
-Theorem wp_lhs_member : forall ty e f Q,
-    wp_lhs e (fun base free =>
+Theorem wp_lval_member : forall ty e f Q,
+    wp_lval e (fun base free =>
         with_addr (_offsetL (_field f) (_eq base)) (fun addr => Q addr free))
-    |-- wp_lhs (Emember e f ty) Q.
+    |-- wp_lval (Emember e f ty) Q.
 Proof.
-  intros. rewrite <- wp_lhs_member.
-  eapply Proper_wp_lhs. red. red. intros.
+  intros. rewrite <- wp_lval_member.
+  eapply Proper_wp_lval. red. red. intros.
   rewrite with_addr_defn. reflexivity.
 Qed.
 
-Theorem wp_lhs_subscript : forall e i t Q,
-    wp_rhs e (fun base free =>
-        wp_rhs i (fun idx free' =>
+Theorem wp_lval_subscript : forall e i t Q,
+    wp_prval e (fun base free =>
+        wp_prval i (fun idx free' =>
           Exists i, [| idx = Vint i |] **
           with_addr (_offsetL (_sub (drop_qualifiers t) i) (_eq base)) (fun addr => Q addr (free' ** free))))
-      |-- wp_lhs (Esubscript e i t) Q.
+      |-- wp_lval (Esubscript e i t) Q.
 Proof.
-  intros. rewrite <- wp_lhs_subscript.
-  eapply Proper_wp_rhs; red; red; intros.
-  eapply Proper_wp_rhs; red; red; intros.
+  intros. rewrite <- wp_lval_subscript.
+  eapply Proper_wp_prval; red; red; intros.
+  eapply Proper_wp_prval; red; red; intros.
   lift_ex_l fail.
   rewrite with_addr_defn.
   work. eapply landL1. reflexivity.
   eapply landL2. reflexivity.
 Qed.
 
-Lemma wp_rhs_unop_wp : forall o e ty Q,
-    wp_rhs e (fun v free =>
-      wp_eval_unop o (drop_qualifiers (type_of e)) (drop_qualifiers ty) v (fun v' => Q v' free))
-    |-- wp_rhs (Eunop o e ty) Q.
+(* primitive operators *)
+
+Lemma wp_prval_unop_wp : forall o e ty Q,
+    wp_prval e (fun v free =>
+      wp_eval_unop o (erase_qualifiers (type_of e)) (erase_qualifiers ty) v (fun v' => Q v' free))
+    |-- wp_prval (Eunop o e ty) Q.
 Proof.
   intros.
   setoid_rewrite wp_eval_unop_defn.
-  eapply wp_rhs_unop.
+  eapply wp_prval_unop.
 Qed.
 
-Lemma wp_rhs_binop_wp : forall o e1 e2 ty Q,
-    wp_rhs e1 (fun v1 free1 =>
-      wp_rhs e2 (fun v2 free2 =>
-        wp_eval_binop o (drop_qualifiers (Typing.type_of e1)) (drop_qualifiers (Typing.type_of e2)) (drop_qualifiers ty) v1 v2 (fun v' => Q v' (free1 ** free2))))
-    |-- wp_rhs (Ebinop o e1 e2 ty) Q.
+Lemma wp_prval_binop_wp : forall o e1 e2 ty Q,
+    wp_prval e1 (fun v1 free1 =>
+      wp_prval e2 (fun v2 free2 =>
+        wp_eval_binop o (erase_qualifiers (Typing.type_of e1)) (erase_qualifiers (Typing.type_of e2)) (erase_qualifiers ty) v1 v2 (fun v' => Q v' (free1 ** free2))))
+    |-- wp_prval (Ebinop o e1 e2 ty) Q.
 Proof.
   intros.
   setoid_rewrite wp_eval_binop_defn.
-  apply wp_rhs_binop.
+  apply wp_prval_binop.
 Qed.
 
-Lemma wp_lhs_preinc_wp : forall e ty Q,
+Lemma wp_lval_preinc_wp : forall e ty Q,
     match companion_type (Typing.type_of e) with
     | Some cty =>
-    wp_lhs e (fun a free =>
+    wp_lval e (fun a free =>
       Exists v',
-        _at (_eq a) (tprim (drop_qualifiers ty) v') **
-        wp_eval_binop Badd (drop_qualifiers (Typing.type_of e)) cty (drop_qualifiers ty) v' (Vint 1%Z) (fun v'' =>
-          _at (_eq a) (tprim (drop_qualifiers ty) v'') -* Q a free))
+        _at (_eq a) (tprim (erase_qualifiers ty) v') **
+        wp_eval_binop Badd (erase_qualifiers (Typing.type_of e)) cty (erase_qualifiers ty) v' (Vint 1%Z) (fun v'' =>
+          _at (_eq a) (tprim (erase_qualifiers ty) v'') -* Q a free))
     | None => lfalse
     end
-    |-- wp_lhs (Epreinc e ty) Q.
+    |-- wp_lval (Epreinc e ty) Q.
 Proof.
   intros.
-  rewrite <-wp_lhs_preinc.
+  rewrite <-wp_lval_preinc.
   destruct (companion_type (type_of e)); auto.
-  eapply Proper_wp_lhs; red; red; intros.
+  eapply Proper_wp_lval; red; red; intros.
   setoid_rewrite wp_eval_binop_defn.
   work.
 Qed.
 
-Lemma wp_lhs_predec_wp : forall e ty Q,
+Lemma wp_lval_predec_wp : forall e ty Q,
     match companion_type (Typing.type_of e) with
     | Some cty =>
-    wp_lhs e (fun a free =>
+    wp_lval e (fun a free =>
       Exists v',
-        _at (_eq a) (tprim (drop_qualifiers ty) v') **
-        wp_eval_binop Bsub (drop_qualifiers (Typing.type_of e)) cty (drop_qualifiers ty) v' (Vint 1%Z) (fun v'' =>
-          _at (_eq a) (tprim (drop_qualifiers ty) v'') -* Q a free))
+        _at (_eq a) (tprim (erase_qualifiers ty) v') **
+        wp_eval_binop Bsub (erase_qualifiers (Typing.type_of e)) cty (erase_qualifiers ty) v' (Vint 1%Z) (fun v'' =>
+          _at (_eq a) (tprim (erase_qualifiers ty) v'') -* Q a free))
     | None => lfalse
     end
-    |-- wp_lhs (Epredec e ty) Q.
+    |-- wp_lval (Epredec e ty) Q.
 Proof.
   intros.
-  rewrite <-wp_lhs_predec.
+  rewrite <-wp_lval_predec.
   destruct (companion_type (type_of e)); auto.
-  eapply Proper_wp_lhs; red; red; intros.
+  eapply Proper_wp_lval; red; red; intros.
   setoid_rewrite wp_eval_binop_defn.
   work.
 Qed.
 
-Lemma wp_rhs_postinc_wp : forall e ty Q,
+Lemma wp_prval_postinc_wp : forall e ty Q,
     match companion_type (type_of e) with
     | Some cty =>
-    wp_lhs e (fun a free =>
+    wp_lval e (fun a free =>
       Exists v',
-        _at (_eq a) (tprim (drop_qualifiers ty) v') **
-        wp_eval_binop Badd (drop_qualifiers (Typing.type_of e)) cty (drop_qualifiers ty) v' (Vint 1%Z) (fun v'' =>
-          _at (_eq a) (tprim (drop_qualifiers ty) v'') -* Q v' free))
+        _at (_eq a) (tprim (erase_qualifiers ty) v') **
+        wp_eval_binop Badd (erase_qualifiers (Typing.type_of e)) cty (erase_qualifiers ty) v' (Vint 1%Z) (fun v'' =>
+          _at (_eq a) (tprim (erase_qualifiers ty) v'') -* Q v' free))
     | None => lfalse
     end
-    |-- wp_rhs (Epostinc e ty) Q.
+    |-- wp_prval (Epostinc e ty) Q.
 Proof.
   intros.
-  rewrite <-wp_rhs_postinc.
+  rewrite <-wp_prval_postinc.
   destruct (companion_type (type_of e)); auto.
-  eapply Proper_wp_lhs; red; red; intros.
+  eapply Proper_wp_lval; red; red; intros.
   setoid_rewrite wp_eval_binop_defn.
   work.
 Qed.
 
-Lemma wp_rhs_postdec_wp : forall e ty Q,
+Lemma wp_prval_postdec_wp : forall e ty Q,
     match companion_type (type_of e) with
     | Some cty =>
-    wp_lhs e (fun a free =>
+    wp_lval e (fun a free =>
       Exists v',
-        _at (_eq a) (tprim (drop_qualifiers ty) v') **
-        wp_eval_binop Bsub (drop_qualifiers (Typing.type_of e)) cty (drop_qualifiers ty) v' (Vint 1%Z) (fun v'' =>
-          _at (_eq a) (tprim (drop_qualifiers ty) v'') -* Q v' free))
+        _at (_eq a) (tprim (erase_qualifiers ty) v') **
+        wp_eval_binop Bsub (erase_qualifiers (Typing.type_of e)) cty (erase_qualifiers ty) v' (Vint 1%Z) (fun v'' =>
+          _at (_eq a) (tprim (erase_qualifiers ty) v'') -* Q v' free))
     | None => lfalse
     end
-    |-- wp_rhs (Epostdec e ty) Q.
+    |-- wp_prval (Epostdec e ty) Q.
 Proof.
   intros.
-  rewrite <-wp_rhs_postdec.
+  rewrite <-wp_prval_postdec.
   destruct (companion_type (type_of e)); auto.
-  eapply Proper_wp_lhs; red; red; intros.
+  eapply Proper_wp_lval; red; red; intros.
   setoid_rewrite wp_eval_binop_defn.
   work.
 Qed.
+
+*)
 
 End with_resolve.
