auto-theories/auto/vc_rw.v
@@ -10,7 +10,7 @@ From Cpp Require Auto.Lemmas Auto.type Auto.vc.
 From Cpp.Auto Require Export Discharge Definitions.
 
 Ltac simplify_simpl :=
-  try unfold finish;
+  try unfold SP;
   simpl k_return;
   simpl k_continue;
   simpl k_break;
@@ -21,83 +21,103 @@ Ltac simplify_simpl :=
   unfold wp_ctor ;
   simpl wpe;
   simpl wps;
-  simpl wpi_init;
   simpl wpis;
   simpl wpds;
+  simpl wp_args;
   simpl offset_for ;
+  simpl drop_qualifiers;
+  simpl erase_qualifiers;
+  simpl is_aggregate;
+  simpl is_pointer;
   simpl wp_block;
   simpl companion_type.
 
-Ltac simplify_wp_rhs e :=
+Ltac simplify_wp_prval e :=
   lazymatch e with
-  | Eatomic _ _ _ => rewrite <- wp_rhs_atomic
-  | Ebinop _ ?e1 _ _ => rewrite <- wp_rhs_binop; continue_rhs e1
-  | Eunop _ ?e _ => rewrite <- wp_rhs_unop; continue_rhs e
-  | Ebool _ => rewrite <- wp_rhs_bool
-  | Eseqand ?e1 _ _ => rewrite <- wp_rhs_seqand; continue_rhs e1
-  | Eseqor ?e1 _ _ => rewrite <- wp_rhs_seqor; continue_rhs e1
-  | Eint _ _ => rewrite <- wp_rhs_int
-  | Eaddrof ?e _ => rewrite <- wp_rhs_addrof; continue_lhs e
-  | Ecast (CCcast Cl2r) (Lvalue, Emember ?o _ _) _ => rewrite <- Lemmas.wp_rhs_dot; continue_lhs o
-  | Ecast (CCcast Cl2r) (Lvalue, Evar (Lname _) _) _ => rewrite <- Lemmas.wp_rhs_local
-  | Ecast (CCcast Cl2r) (Lvalue, ?e) _ => rewrite <- Lemmas.wp_rhs_cast_l2r; continue_lhs e
-  | Ecast (CCcast Carray2pointer) (Lvalue, ?e) _ => rewrite <- wp_rhs_cast_array2pointer; continue_lhs e
+  | Eatomic _ _ _ => rewrite <- wp_prval_atomic
+  | Ebinop _ ?e1 _ _ => rewrite <- wp_prval_binop; continue_prval e1
+  | Eunop _ ?e _ => rewrite <- wp_prval_unop; continue_prval e
+  | Ebool _ => rewrite <- wp_prval_bool
+  | Eseqand ?e1 _ _ => rewrite <- wp_prval_seqand; continue_prval e1
+  | Eseqor ?e1 _ _ => rewrite <- wp_prval_seqor; continue_prval e1
+  | Eint _ _ => rewrite <- wp_prval_int
+  | Eaddrof ?e _ => rewrite <- wp_prval_addrof; continue_lval e
+  | Ecast (CCcast Cl2r) (Lvalue, Emember ?o _ _) _ => rewrite <- Lemmas.wp_prval_dot; continue_lval o
+  | Ecast (CCcast Cl2r) (Lvalue, Evar (Lname _) _) _ => rewrite <- Lemmas.wp_prval_local
+  | Ecast (CCcast Cl2r) (Lvalue, ?e) _ => rewrite <- Lemmas.wp_prval_cast_l2r_l; continue_lval e
+  | Ecast (CCcast Cl2r) (Xvalue, ?e) _ => rewrite <- Lemmas.wp_prval_cast_l2r_x; continue_xval e
+  | Ecast (CCcast Carray2pointer) (Lvalue, ?e) _ => rewrite <- wp_prval_cast_array2pointer; continue_lval e
   | Ecast ?c (Rvalue, ?e) _ =>
     lazymatch c with
-    | CCcast Cintegral => rewrite <- wp_rhs_cast_integral
-    | CCcast Cint2bool => rewrite <- wp_rhs_cast_int2bool
-    | CCcast Cptr2bool => rewrite <- wp_rhs_cast_ptr2bool
-    | CCcast Cnull2ptr => rewrite <- wp_rhs_cast_null
-    | CCcast Cnoop => rewrite <- Lemmas.wp_rhs_cast_noop
-    | CCcast Cbitcast => rewrite <- wp_rhs_cast_bitcast
-    | Cuser _ => rewrite <- wp_rhs_cast_user
-    | Creinterpret _ => rewrite <- wp_rhs_cast_reinterpret
-    end; continue_rhs e
+    | CCcast Cintegral => rewrite <- wp_prval_cast_integral
+    | CCcast Cint2bool => rewrite <- wp_prval_cast_int2bool
+    | CCcast Cptr2bool => rewrite <- wp_prval_cast_ptr2bool
+    | CCcast Cnull2ptr => rewrite <- wp_prval_cast_null
+    | CCcast Cnoop => rewrite <- wp_prval_cast_noop
+    | CCcast Cbitcast => rewrite <- wp_prval_cast_bitcast
+    | Cuser _ => rewrite <- wp_prval_cast_user
+    | Creinterpret _ => rewrite <- wp_prval_cast_reinterpret
+    end; continue_prval e
   | Enull => rewrite <- wp_null
-  | Ethis _ => rewrite <- wp_rhs_this
-  | Ealign_of (inl _) _ => rewrite <- wp_rhs_alignof
-  | Ealign_of (inr _) _ => rewrite <- wp_rhs_alignof_e
-  | Esize_of (inl _) _ => rewrite <- wp_rhs_sizeof
-  | Esize_of (inr _) _ => rewrite <- wp_rhs_sizeof_e
-  | Epostinc _ _ => rewrite <- wp_rhs_postinc; simpl
-  | Epostdec _ _ => rewrite <- wp_rhs_postdec; simpl
-  | Eandclean ?e _ => rewrite <- wp_rhs_clean; continue_rhs e
+  | Ethis _ => rewrite <- wp_prval_this
+  | Ealign_of (inl _) _ => rewrite <- wp_prval_alignof
+  | Ealign_of (inr _) _ => rewrite <- wp_prval_alignof_e
+  | Esize_of (inl _) _ => rewrite <- wp_prval_sizeof
+  | Esize_of (inr _) _ => rewrite <- wp_prval_sizeof_e
+  | Epostinc _ _ => rewrite <- wp_prval_postinc; simpl
+  | Epostdec _ _ => rewrite <- wp_prval_postdec; simpl
+  | Eandclean ?e _ => rewrite <- wp_prval_clean; continue_prval e
   end
 
-with simplify_wp_lhs e :=
+with simplify_wp_xval e :=
   lazymatch e with
-  | Eassign (Emember ?o _ _) _ _ => rewrite <- Lemmas.wp_lhs_assign_member; continue_lhs o
-  | Eassign ?l _ _ => rewrite <- wp_lhs_assign; continue_lhs l
-  | Eassign_op _ _ _ _ => rewrite <- wp_lhs_bop_assign
-  | Evar (Lname _) _ => rewrite <- wp_lhs_lvar
-  | Evar (Gname _) _ => rewrite <- wp_lhs_gvar
-  | Ederef ?e _ => rewrite <- wp_lhs_deref; continue_rhs e
-  | Ecast (CCcast Cnoop) (Lvalue, ?e) _ => rewrite <- Lemmas.wp_lhs_cast_noop; continue_lhs e
-  | Emember ?e _ _ => rewrite <- wp_lhs_member; continue_lhs e
-  | Epreinc _ _ => rewrite <- wp_lhs_preinc; simpl
-  | Epredec _ _ => rewrite <- wp_lhs_predec; simpl
-  | Eif ?e _ _ _ => rewrite <- Lemmas.wp_lhs_condition; continue_rhs e
-  | Ematerialize_temp ?e _ => rewrite <- wp_lhs_temp; continue_rhs e
-  | Esubscript ?e _ _ => rewrite <- wp_lhs_subscript; continue_rhs e
+  | _ => idtac
   end
-with continue_rhs e := try (simplify_simpl; simplify_wp_rhs e)
-with continue_lhs e := try (simplify_simpl; simplify_wp_lhs e)
+
+with simplify_wp_lval e :=
+  lazymatch e with
+  | Eassign (Emember ?o _ _) _ _ => rewrite <- Lemmas.wp_lval_assign_member; continue_lval o
+  | Eassign ?l _ _ => rewrite <- wp_lval_assign; continue_lval l
+  | Eassign_op _ _ _ _ => rewrite <- wp_lval_bop_assign
+  | Evar (Lname _) _ => rewrite <- wp_lval_lvar
+  | Evar (Gname _) _ => rewrite <- wp_lval_gvar
+  | Ederef ?e _ => rewrite <- wp_lval_deref; continue_prval e
+  | Ecast (CCcast Cnoop) (Lvalue, ?e) _ =>
+    rewrite <- wp_lval_cast_noop; continue_lval e
+  | Ecast (CCcast Cnoop) (Xvalue, ?e) _ =>
+    rewrite <- wp_lval_xval_cast_noop; continue_lval e
+  | Emember ?e _ _ => rewrite <- wp_lval_member; continue_lval e
+  | Epreinc _ _ => rewrite <- wp_lval_preinc; simpl
+  | Epredec _ _ => rewrite <- wp_lval_predec; simpl
+  | Eif ?e _ _ _ => rewrite <- Lemmas.wp_lval_condition; continue_prval e
+  | Ematerialize_temp ?e _ => rewrite <- wp_lval_temp; continue_prval e
+  | Esubscript ?e _ _ => rewrite <- wp_lval_subscript; continue_prval e
+  end
+with simplify_wp_init e :=
+  (rewrite <- wp_init_wp_init')
+
+with continue_prval e := try (simplify_simpl; simplify_wp_prval e)
+with continue_lval e := try (simplify_simpl; simplify_wp_lval e)
+with continue_xval e := try (simplify_simpl; simplify_wp_xval e)
+with continue_init e := try (simplify_simpl; simplify_wp_init e)
 .
 
+(*
 Ltac simplify_wpe e :=
   lazymatch e with
   | Ecast (CCcast Cnoop) (_, ?e) _ => rewrite <- wpe_cast_noop; try (simplify_simpl; simplify_wpe e)
   end.
+*)
 
 Ltac simplify_wp_ e :=
   lazymatch e with
   | Sseq _ => rewrite <- wp_seq
-  | Sreturn (Some (Lvalue, ?e)) => rewrite <- Lemmas.wp_return_lhs; try (simplify_simpl; simplify_wp_lhs e)
-  | Sreturn (Some (Rvalue, ?e)) => rewrite <- Lemmas.wp_return_rhs; try (simplify_simpl; simplify_wp_rhs e)
+  | Sreturn (Some (Lvalue, ?e)) => rewrite <- Lemmas.wp_return_lval; try (simplify_simpl; simplify_wp_lval e)
+  | Sreturn (Some (Rvalue, ?e)) => rewrite <- Lemmas.wp_return_rval; simpl is_aggregate; try (simplify_simpl; simplify_wp_prval e)
   | Sreturn None => rewrite <- wp_return_void
   | Sexpr _ _ => rewrite <- wp_expr
   | Sif (Some _) _ _ _ => rewrite <- wp_if_decl
-  | Sif None ?e _ _ => rewrite <- wp_if; try (simplify_simpl; simplify_wp_rhs e)
+  | Sif None ?e _ _ => rewrite <- wp_if; try (simplify_simpl; simplify_wp_prval e)
   | Sfor (Some _) _ _ _ => rewrite <- wp_for_init
   | Swhile (Some _) _ _ => rewrite <- wp_while_decl
   | Scontinue => rewrite <- wp_continue
@@ -118,6 +138,7 @@ Ltac simplify_wp_decl t :=
   | Treference _ => rewrite <- Lemmas.wp_decl_reference
   end.
 
+
 Ltac simplify_wp' g :=
   lazymatch g with
   | ?g1 ** ?g2 => first [ simplify_wp' g1 | simplify_wp' g2 ]
@@ -126,9 +147,10 @@ Ltac simplify_wp' g :=
   | lexists (fun _x : _ => ?g) _ => simplify_wp' g
   | lforall (fun _x : _ => ?g) _ => simplify_wp' g
   | wp _ _ ?e _ => simplify_wp_ e
-  | wp_rhs _ _ ?e _ => simplify_wp_rhs e
-  | wp_lhs _ _ ?e _ => simplify_wp_lhs e
-  | wp_decl _ _ _ ?t _ _ _ => simplify_wp_decl t
+  | wp_prval _ _ ?e _ => simplify_wp_prval e
+  | wp_lval _ _ ?e _ => simplify_wp_lval e
+  | wp_decl _ _ _ ?t _ _ _ _ => simplify_wp_decl t
+  | @wp_init _ _ _ _ _ ?e _ => simplify_wp_init e
   | wpd _ _ _ _ _ _ => rewrite <- wpd_deinit
   | wpi _ _ _ _ _ _ => rewrite <- wpi_initialize
   end.
@@ -148,22 +170,27 @@ Ltac simplifying :=
       lazymatch goal with
       | |- _ |-- ?R =>
         match R with
-        | context [ wp_rhs _ _ (Ecall _ _ _) _ ] =>
-          perm_right ltac:(idtac; simple eapply Lemmas.wp_call_glob;
+        | context [ wp_prval _ _ (Ecall _ _ _) _ ] =>
+          perm_right ltac:(idtac; simple eapply Lemmas.wp_prval_call_glob;
                            [ exact I | find_spec | simpl wps ])
-        | context [ wp_rhs _ _ (Emember_call _ _ _ _ _) _ ] =>
-          try_it Lemmas.wp_member_call_glob
-        | context [ wp_rhs _ _ (Econstructor _ _ _) _ ] =>
-          perm_right ltac:(idtac; simple eapply Lemmas.wp_constructor_glob;
-                           [ find_spec | simpl wps ])
-        | context [ wp_decl _ _ _ (Tref _) _ _ ] =>
-          perm_right ltac:(idtac; simple eapply Lemmas.wp_decl_class;
-                           [ find_spec | find_spec | simpl wps ])
-        | context [ @destroy _ _ _ _ _ _ ] =>
-          perm_right ltac:(idtac; simple eapply Lemmas.wp_destroy;
-                           [ find_spec | simpl ])
-        | context [ @wp_rhs _ _ _ (Econst_ref _ _) _ ] =>
-          perm_right ltac:(idtac; simple eapply Lemmas.wp_rhs_const;
+        | context [ wp_xval _ _ (Ecall _ _ _) _ ] =>
+          perm_right ltac:(idtac; simple eapply Lemmas.wp_xval_call_glob;
+                           [ exact I | find_spec | simpl wps ])
+        | context [ wp_prval _ _ (Emember_call _ _ _ _ _) _ ] =>
+          try_it Lemmas.wp_prval_member_call_glob
+        | context [ wp_xval _ _ (Emember_call _ _ _ _ _) _ ] =>
+          try_it Lemmas.wp_xval_member_call_glob
+        (* | context [ wp_prval _ _ (Econstructor _ _ _) _ ] => *)
+        (*   perm_right ltac:(idtac; simple eapply Lemmas.wp_constructor_glob; *)
+        (*                    [ find_spec | simpl wps ]) *)
+        (* | context [ wp_decl _ _ _ (Tref _) _ _ ] => *)
+        (*   perm_right ltac:(idtac; simple eapply Lemmas.wp_decl_class; *)
+        (*                    [ find_spec | find_spec | simpl wps ]) *)
+        (* | context [ @destroy _ _ _ _ _ _ ] => *)
+        (*   perm_right ltac:(idtac; simple eapply Lemmas.wp_destroy; *)
+        (*                    [ find_spec | simpl ]) *)
+        | context [ @wp_prval _ _ _ (Econst_ref _ _) _ ] =>
+          perm_right ltac:(idtac; simple eapply Lemmas.wp_prval_const;
                            [ solve [ perm_left ltac:(idtac; eapply Lemmas.exactly_this_one) ] | reflexivity | ])
         end
       end
