auto-theories/auto/vc_rws.v
@@ -1,0 +1,278 @@
+(*
+ * Copyright (C) BedRock Systems Inc. 2019 Gregory Malecha
+ *
+ * SPDX-License-Identifier:AGPL-3.0-or-later
+ *)
+(* Automation for code *)
+Require Import LtacIter.LtacIter.
+
+From Cpp Require Export Ast Sem.
+Require Cpp.Auto.Lemmas.
+
+From Cpp.Auto Require Export Discharge Definitions.
+
+Global Opaque wp_decl.
+
+(* we are working in a fairly rich separation logic, however, the fragment that
+ * shows up in practice is relatively small.
+ *)
+Create HintDb wp_pre discriminated.
+
+Hint Resolve Lemmas.wp_prval_dot Lemmas.wp_prval_local (* Lemmas.wp_lval_assign_member *) : wp_pre.
+
+Local Ltac t :=
+  discharge fail idtac fail fail idtac.
+
+Ltac find_left tac :=
+  let rec perm :=
+      lazymatch goal with
+      | |- (?A ** ?B) ** ?C |-- _ => first
+          [ simple eapply Discharge.focus_ll; perm
+          | simple eapply Discharge.focus_lr; perm ]
+      | |- _ => tac
+      end
+  in
+  lazymatch goal with
+  | |- _ ** _ |-- _ => first
+    [ perm | simple eapply Discharge.focus_lswap; perm ]
+  | |- empSP |-- _ => fail
+  | |- _ |-- _ => simple eapply Discharge.focus_lstart; tac
+  end.
+
+(* this tactic solves goals of the form
+ *
+ *   F |-- |> cglob' f ti s ** ltrue
+ *
+ * which arise from various forms of calls.
+ *)
+Ltac find_spec :=
+  let try_this_one :=
+      first [ simple eapply Lemmas.cglob_by_cglob_gen;
+              solve [ reflexivity
+                    | eapply (@Lemmas.unify_SFunction _ _ _ _ _ _ eq_refl eq_refl eq_refl) ]
+            | simple eapply Lemmas.cglob_by_ti_cglob_gen;
+              solve [ reflexivity
+                    | eapply (@Lemmas.unify_SFunction _ _ _ _ _ _ eq_refl eq_refl eq_refl) ]
+            | simple eapply Lemmas.cglob_by_later_cglob_gen;
+              solve [ reflexivity
+                    | eapply (@Lemmas.unify_SFunction _ _ _ _ _ _ eq_refl eq_refl eq_refl) ]
+            | simple eapply Lemmas.cglob_by_later_ti_cglob_gen;
+              solve [ reflexivity
+                    | eapply (@Lemmas.unify_SFunction _ _ _ _ _ _ eq_refl eq_refl eq_refl) ]
+            | simple eapply Lemmas.cglob_by_make_signature_ti_gen;
+              [ reflexivity
+              | solve [ reflexivity
+                      | eapply (@Lemmas.unify_SFunction _ _ _ _ _ _ eq_refl eq_refl eq_refl) ] ]
+            | simple eapply Lemmas.cglob_by_later_make_signature_ti_gen;
+              [ reflexivity
+              | solve [ reflexivity
+                      | eapply (@Lemmas.unify_SFunction _ _ _ _ _ _ eq_refl eq_refl eq_refl) ] ]
+            ]
+  in
+  solve [ find_left try_this_one ].
+
+Create HintDb wp_all discriminated.
+
+Hint Rewrite <-
+     @wp_seq
+     Lemmas.wp_return_lval
+     Lemmas.wp_return_rval
+     Lemmas.wp_return_xval
+     @wp_return_void @wp_expr
+     @wp_if_decl
+     @wp_if
+     @wp_for_init
+     @wp_while_decl
+     @wp_continue
+     @wp_break
+     Lemmas.wp_skip
+     @wp_prval_atomic
+
+     @wp_prval_binop
+     @wp_prval_unop
+     @wp_prval_bool
+     @wp_lval_assign
+     @wp_lval_bop_assign
+     @wp_lval_lvar
+     @wp_lval_gvar
+     @wp_prval_seqand
+     @wp_prval_seqor
+     @wp_prval_int
+     @wp_lval_deref
+     @wp_prval_addrof
+     Lemmas.wp_prval_cast_l2r_l
+     Lemmas.wp_prval_cast_l2r_x
+     @wp_prval_cast_integral
+     @wp_prval_cast_int2bool
+     @wp_prval_cast_ptr2bool
+     @wp_prval_cast_null
+     @wp_xval_cast_noop
+     @wp_lval_cast_noop
+     @wp_xval_lval_cast_noop
+     @wp_lval_xval_cast_noop
+     @wp_prval_cast_noop
+     @wp_prval_cast_bitcast
+     @wp_prval_cast_array2pointer
+     @wp_null
+     @wp_lval_member
+     @wp_prval_this
+     @wp_prval_alignof
+     @wp_prval_alignof_e
+     @wp_prval_sizeof
+     @wp_prval_sizeof_e
+     @wp_prval_postinc
+     @wp_prval_postdec
+     @wp_lval_preinc
+     @wp_lval_predec
+     Lemmas.wp_lval_condition
+     Lemmas.wp_prval_condition
+     @wp_prval_cast_user
+     @wp_prval_cast_reinterpret
+     @wp_prval_clean
+     @wp_lval_temp
+     @wp_lval_subscript
+
+     Lemmas.wp_decl_mut
+     Lemmas.wp_decl_const
+     Lemmas.wp_decl_int
+     Lemmas.wp_decl__int
+     Lemmas.wp_decl__int32
+     Lemmas.wp_decl__ulong
+     Lemmas.wp_decl_char
+     Lemmas.wp_decl_pointer
+     Lemmas.wp_decl_reference
+
+     Lemmas.wp_init_mut
+
+     @wpd_deinit
+  : wp_all.
+Hint Rewrite <- @wp_init_clean : wp_all.
+Hint Rewrite <- @wp_init_const @wp_init_mut : wp_all.
+Hint Rewrite <- @wp_xval_temp : wp_all.
+Hint Rewrite <- @wp_init_cast_noop : wp_all.
+Hint Rewrite <- @wp_init_bind_temp : wp_all.
+Hint Rewrite <- @Lemmas.wp_prval_cast_tovoid : wp_all.
+Hint Rewrite <- @wp_xval_member @wp_prval_member @wp_lval_member : wp_all.
+
+Hint Rewrite <- @Lemmas.wp_rval_xval_materialize @wp_prval_materialize : wp_all.
+
+
+Hint Rewrite <- @Lemmas.wpi_initialize : wp_all.
+
+
+Require Import Coq.Classes.Morphisms.
+
+(* note(gmm): the following morphisms seem to be necessary *)
+Global Instance lexists_ok : Proper (pointwise_relation val (Basics.flip lentails) ==> Basics.flip lentails) (@lexists mpred _ _).
+Proof.
+  red. red. intros. red.
+  eapply lexists_lentails_m.
+  eapply H.
+Qed.
+Global Instance lentails_ok : Proper (lentails ==> Basics.flip lentails ==> Basics.flip Basics.impl) (@lentails mpred _).
+Proof.
+  red. red. red. intros. red. intros. red.
+  intros.
+  etransitivity. eauto. etransitivity; eauto.
+Qed.
+
+Global Instance lentails_ok_R : forall P, Proper (lentails --> Basics.flip Basics.impl) (@lentails mpred _ P).
+Proof.
+  red. red. red. intros. red. intros.
+  etransitivity. eauto. eapply H.
+Qed.
+Global Instance : subrelation eq (Basics.flip (@lentails mpred _)).
+Proof. repeat red. intros. subst. reflexivity. Qed.
+Global Instance : Transitive (Basics.flip (@lentails mpred _)).
+Proof. do 2 red. intros. etransitivity. eapply H0. eapply H. Qed.
+
+Global Instance :
+  forall (resolve : genv) (ti : thread_info) (r : region) (e : Stmt) K,
+  @Proper mpred
+    (@lentails mpred ILogicOps_mpred)
+    (@wp resolve ti r e K).
+Proof. red. intros. reflexivity. Qed.
+Global Instance : forall P, Proper (@lentails mpred _ --> Basics.flip Basics.impl) (@lentails mpred _ P).
+Proof. red. red. red. red. intros. etransitivity; [ eapply H0 | eapply H ]. Qed.
+
+
+Global Instance : Proper (lentails ==> Basics.flip lentails ==> Basics.flip lentails) (@wandSP mpred _).
+Proof. red. red. red. red. unfold Basics.flip. intros.
+       rewrite H. rewrite H0. reflexivity.
+Qed.
+Global Instance : forall P, Proper (Basics.flip lentails ==> Basics.flip lentails) (@wandSP mpred _ P).
+Proof. red. red. red. unfold Basics.flip. intros.
+       rewrite H. reflexivity.
+Qed.
+Global Instance lforall_ok : Proper (pointwise_relation val (Basics.flip lentails) ==> Basics.flip lentails) (@lforall mpred _ _).
+Proof. red. red. red. intros.
+       eapply lforall_lentails_m. apply H.
+Qed.
+
+Declare Reduction red_wpe :=
+  cbn beta iota zeta delta [
+        drop_qualifiers erase_qualifiers
+        wp_args wp_block wp_decls wpAny wpe wp_initialize
+        Qmut Qconst T_int
+        is_aggregate is_pointer type_of
+        k_normal k_break k_return k_continue
+        Kloop Kseq Kfree Kat_exit val_return void_return
+        init_path init_type init_init Wp.SP ].
+
+Declare Reduction red_wpe_n :=
+  cbv beta iota zeta delta [ Wp.SP ].
+
+Remove Hints Equivalence_Symmetric Equivalence_PER SepAlg.sa_type : typeclass_instances.
+Global Instance : Params (@sepSP) 2.
+Global Instance : Params (@land) 2.
+Global Instance : Params (@lor) 2.
+Global Instance : Params (@wandSP) 2.
+Global Instance : Params (@empSP) 0.
+Global Instance : Params (@ltrue) 0.
+Global Instance : Params (@lfalse) 0.
+
+
+Ltac simplify_all :=
+  rewrite_strat (topdown (hints wp_all; eval red_wpe_n; eval red_wpe)).
+
+Ltac simplify_one :=
+  rewrite_strat (outermost (hints wp_all; eval red_wpe_n; eval red_wpe)).
+
+(*
+Require Import Coq.Strings.String.
+Require Import Coq.ZArith.ZArith.
+Local Open Scope string_scope.
+
+Goal forall resolve ti r Q,
+    |-- wp_lval (resolve:=resolve) ti r
+        (Eassign
+           (Ederef
+              (Ecast (CCcast Cl2r)
+                     (Lvalue, Eassign
+                                (Evar
+                                   (Lname  "x")
+                                   (Qmut
+                                      (Tpointer
+                                         (Qmut T_int))))
+                                (Eaddrof
+                                   (Evar
+                                      (Lname  "y")
+                                      (Qmut T_int))
+                                   (Qmut
+                                      (Tpointer
+                                         (Qmut T_int))))
+                                (Qmut
+                                   (Tpointer
+                                      (Qmut T_int))))
+                     (Qmut
+                        (Tpointer
+                           (Qmut T_int))))
+              (Qmut T_int))
+           (Eint 3
+                 (Qmut T_int))
+           (Qmut T_int))%Z Q.
+Proof.
+  intros.
+  Time simplify_all.
+Abort.
+*)
